Variables evaluate properly

BananasLanguage.thy
@@ -41,8 +41,8 @@ fun apply_functor_type :: "type \<Rightarrow> funct \<Rightarrow> type" (infixl 
 | "t \<star> f\<^sub>1 \<Otimes> f\<^sub>2 = (t \<star> f\<^sub>1) \<otimes> (t \<star> f\<^sub>2)"
 | "t \<star> f\<^sub>1 \<Oplus> f\<^sub>2 = (t \<star> f\<^sub>1) \<oplus> (t \<star> f\<^sub>2)"
 
-inductive typecheck\<^sub>e :: "(name \<Rightarrow> type) \<Rightarrow> expr \<Rightarrow> type \<Rightarrow> type \<Rightarrow> bool" (infix "\<turnstile> _ : _ \<rightarrow>" 60)
-      and typecheck\<^sub>v :: "(name \<Rightarrow> type) \<Rightarrow> val \<Rightarrow> type \<Rightarrow> bool" (infix "\<turnstile> _ :" 60) where
+inductive typecheck\<^sub>e :: "(name \<Rightarrow> type \<times> type) \<Rightarrow> expr \<Rightarrow> type \<Rightarrow> type \<Rightarrow> bool" (infix "\<turnstile> _ : _ \<rightarrow>" 60)
+      and typecheck\<^sub>v :: "(name \<Rightarrow> type \<times> type) \<Rightarrow> val \<Rightarrow> type \<Rightarrow> bool" (infix "\<turnstile> _ :" 60) where
   tc_id [simp]: "\<Gamma> \<turnstile> \<epsilon> : t \<rightarrow> t"
 | tc_con [simp]: "\<Gamma> \<turnstile> v : t\<^sub>2 \<Longrightarrow> \<Gamma> \<turnstile> \<kappa> v : t\<^sub>1 \<rightarrow> t\<^sub>2"
 | tc_comp [simp]: "\<Gamma> \<turnstile> f : t\<^sub>2 \<rightarrow> t\<^sub>3 \<Longrightarrow> \<Gamma> \<turnstile> g : t\<^sub>1 \<rightarrow> t\<^sub>2 \<Longrightarrow> \<Gamma> \<turnstile> f \<cdot> g : t\<^sub>1 \<rightarrow> t\<^sub>3"
@@ -61,6 +61,7 @@ inductive typecheck\<^sub>e :: "(name \<Rightarrow> type) \<Rightarrow> expr \<R
 | tc_outj [simp]: "\<Gamma> \<turnstile> \<prec>\<^bsub>F\<^esub> : \<mu> F \<rightarrow> \<mu> F \<star> F"
 | tc_cata [simp]: "\<Gamma> \<turnstile> f : t \<star> F \<rightarrow> t \<Longrightarrow> \<Gamma> \<turnstile> \<lparr> f \<rparr>\<^bsub>F\<^esub> : \<mu> F \<rightarrow> t"
 | tc_ana [simp]: "\<Gamma> \<turnstile> f : t \<rightarrow> t \<star> F \<Longrightarrow> \<Gamma> \<turnstile> \<lbrakk> f \<rbrakk>\<^bsub>F\<^esub> : t \<rightarrow> \<mu> F"
+| tc_var [simp]: "\<Gamma> x = (t\<^sub>1, t\<^sub>2) \<Longrightarrow> \<Gamma> \<turnstile> Var x : t\<^sub>1 \<rightarrow> t\<^sub>2"
 
 | tcv_unit [simp]: "\<Gamma> \<turnstile> UnitV : \<one>"
 | tcv_pair [simp]: "\<Gamma> \<turnstile> v\<^sub>1 : t\<^sub>1 \<Longrightarrow> \<Gamma> \<turnstile> v\<^sub>2 : t\<^sub>2 \<Longrightarrow> \<Gamma> \<turnstile> PairV v\<^sub>1 v\<^sub>2 : t\<^sub>1 \<otimes> t\<^sub>2"
@@ -87,6 +88,7 @@ inductive_cases [elim]: "\<Gamma> \<turnstile> \<prec>\<^bsub>F\<^esub> : t \<ri
 inductive_cases [elim]: "\<Gamma> \<turnstile> \<succ>\<^bsub>F\<^esub> : t \<rightarrow> t'"
 inductive_cases [elim]: "\<Gamma> \<turnstile> \<lparr> f \<rparr>\<^bsub>F\<^esub> : t \<rightarrow> t'"
 inductive_cases [elim]: "\<Gamma> \<turnstile> \<lbrakk> f \<rbrakk>\<^bsub>F\<^esub> : t \<rightarrow> t'"
+inductive_cases [elim]: "\<Gamma> \<turnstile> Var x : t \<rightarrow> t'"
 
 inductive_cases [elim]: "\<Gamma> \<turnstile> UnitV : t"
 inductive_cases [elim]: "\<Gamma> \<turnstile> PairV v\<^sub>1 v\<^sub>2 : t"
@@ -94,6 +96,9 @@ inductive_cases [elim]: "\<Gamma> \<turnstile> InrV v : t"
 inductive_cases [elim]: "\<Gamma> \<turnstile> InlV v : t"
 inductive_cases [elim]: "\<Gamma> \<turnstile> FunV e : t"
 inductive_cases [elim]: "\<Gamma> \<turnstile> InjV f v : t"
+
+definition typecheck_context :: "(name \<Rightarrow> type \<times> type) \<Rightarrow> (name \<Rightarrow> expr) \<Rightarrow> bool" (infix "\<tturnstile>" 60) where
+  "\<Gamma> \<tturnstile> \<Lambda> = (\<forall>x t\<^sub>1 t\<^sub>2. \<Gamma> x = (t\<^sub>1, t\<^sub>2) \<longrightarrow> \<Gamma> \<turnstile> \<Lambda> x : t\<^sub>1 \<rightarrow> t\<^sub>2)"
 
 (* evaluation *)
 
@@ -103,30 +108,32 @@ fun apply_functor_expr :: "expr \<Rightarrow> funct \<Rightarrow> expr" (infixl 
 | "e \<bullet> f\<^sub>1 \<Otimes> f\<^sub>2 = (e \<bullet> f\<^sub>1) \<parallel> (e \<bullet> f\<^sub>2)"
 | "e \<bullet> f\<^sub>1 \<Oplus> f\<^sub>2 = (e \<bullet> f\<^sub>1) \<bar> (e \<bullet> f\<^sub>2)"
 
-inductive evaluate :: "expr \<Rightarrow> val \<Rightarrow> expr \<Rightarrow> val \<Rightarrow> bool" (infix "\<cdot> _ \<leadsto> _ \<cdot>" 60) where
-  ev_con [simp]: "\<kappa> v\<^sub>1 \<cdot> v\<^sub>2 \<leadsto> \<epsilon> \<cdot> v\<^sub>1"
-| ev_comp1 [simp]: "g \<cdot> v \<leadsto> g' \<cdot> v' \<Longrightarrow> (f \<cdot> g) \<cdot> v \<leadsto> (f \<cdot> g') \<cdot> v'"
-| ev_comp2 [simp]: "(f \<cdot> \<epsilon>) \<cdot> v \<leadsto> f \<cdot> v"
-| ev_fst [simp]: "\<pi>\<^sub>1 \<cdot> PairV v\<^sub>1 v\<^sub>2 \<leadsto> \<epsilon> \<cdot> v\<^sub>1"
-| ev_snd [simp]: "\<pi>\<^sub>2 \<cdot> PairV v\<^sub>1 v\<^sub>2 \<leadsto> \<epsilon> \<cdot> v\<^sub>2"
-| ev_pair1 [simp]: "f\<^sub>1 \<cdot> v\<^sub>1 \<leadsto> f\<^sub>1' \<cdot> v\<^sub>1' \<Longrightarrow> f\<^sub>1 \<parallel> f\<^sub>2 \<cdot> PairV v\<^sub>1 v\<^sub>2 \<leadsto> f\<^sub>1' \<parallel> f\<^sub>2 \<cdot> PairV v\<^sub>1' v\<^sub>2"
-| ev_pair2 [simp]: "f\<^sub>2 \<cdot> v\<^sub>2 \<leadsto> f\<^sub>2' \<cdot> v\<^sub>2' \<Longrightarrow> \<epsilon> \<parallel> f\<^sub>2 \<cdot> PairV v\<^sub>1 v\<^sub>2 \<leadsto> \<epsilon> \<parallel> f\<^sub>2' \<cdot> PairV v\<^sub>1 v\<^sub>2'"
-| ev_pair3 [simp]: "\<epsilon> \<parallel> \<epsilon> \<cdot> PairV v\<^sub>1 v\<^sub>2 \<leadsto> \<epsilon> \<cdot> PairV v\<^sub>1 v\<^sub>2"
-| ev_tup [simp]: "\<Theta> \<cdot> v \<leadsto> \<epsilon> \<cdot> PairV v v"
-| ev_inl [simp]: "\<iota>\<^sub>l \<cdot> v \<leadsto> \<epsilon> \<cdot> InlV v"
-| ev_inr [simp]: "\<iota>\<^sub>r \<cdot> v \<leadsto> \<epsilon> \<cdot> InrV v"
-| ev_strl [simp]: "\<Xi> \<cdot> InlV v \<leadsto> \<epsilon> \<cdot> v"
-| ev_strr [simp]: "\<Xi> \<cdot> InrV v \<leadsto> \<epsilon> \<cdot> v"
-| ev_csl [simp]: "f\<^sub>l \<bar> f\<^sub>r \<cdot> InlV v \<leadsto> (\<iota>\<^sub>l \<cdot> f\<^sub>l) \<cdot> v"
-| ev_csr [simp]: "f\<^sub>l \<bar> f\<^sub>r \<cdot> InrV v \<leadsto> (\<iota>\<^sub>r \<cdot> f\<^sub>r) \<cdot> v"
-| ev_dstl [simp]: "\<rhd> \<cdot> PairV (InlV v\<^sub>1) v\<^sub>2 \<leadsto> \<epsilon> \<cdot> InlV (PairV v\<^sub>1 v\<^sub>2)"
-| ev_dstr [simp]: "\<rhd> \<cdot> PairV (InrV v\<^sub>1) v\<^sub>2 \<leadsto> \<epsilon> \<cdot> InrV (PairV v\<^sub>1 v\<^sub>2)"
-| ev_app [simp]: "$ \<cdot> PairV (FunV e) v \<leadsto> e \<cdot> v"
-| ev_arr [simp]: "g \<leftarrow> f \<cdot> FunV e \<leadsto> \<epsilon> \<cdot> FunV (g \<cdot> e \<cdot> f)"
-| ev_inj [simp]: "\<succ>\<^bsub>F\<^esub> \<cdot> v \<leadsto> \<epsilon> \<cdot> InjV F v"
-| ev_outj [simp]: "\<prec>\<^bsub>F\<^esub> \<cdot> InjV F v \<leadsto> \<epsilon> \<cdot> v"
-| ev_cata [simp]: "\<lparr> f \<rparr>\<^bsub>F\<^esub> \<cdot> v \<leadsto> (f \<cdot> \<lparr> f \<rparr>\<^bsub>F\<^esub> \<bullet> F \<cdot> \<prec>\<^bsub>F\<^esub>) \<cdot> v"
-| ev_ana [simp]: "\<lbrakk> f \<rbrakk>\<^bsub>F\<^esub> \<cdot> v \<leadsto> (\<succ>\<^bsub>F\<^esub> \<cdot> \<lbrakk> f \<rbrakk>\<^bsub>F\<^esub> \<bullet> F \<cdot> f) \<cdot> v"
+inductive evaluate :: "(name \<Rightarrow> expr) \<Rightarrow> expr \<Rightarrow> val \<Rightarrow> expr \<Rightarrow> val \<Rightarrow> bool" 
+    (infix "\<turnstile> _ \<cdot> _ \<leadsto> _ \<cdot>" 60) where
+  ev_con [simp]: "\<Lambda> \<turnstile> \<kappa> v\<^sub>1 \<cdot> v\<^sub>2 \<leadsto> \<epsilon> \<cdot> v\<^sub>1"
+| ev_comp1 [simp]: "\<Lambda> \<turnstile> g \<cdot> v \<leadsto> g' \<cdot> v' \<Longrightarrow> \<Lambda> \<turnstile> (f \<cdot> g) \<cdot> v \<leadsto> (f \<cdot> g') \<cdot> v'"
+| ev_comp2 [simp]: "\<Lambda> \<turnstile> (f \<cdot> \<epsilon>) \<cdot> v \<leadsto> f \<cdot> v"
+| ev_fst [simp]: "\<Lambda> \<turnstile> \<pi>\<^sub>1 \<cdot> PairV v\<^sub>1 v\<^sub>2 \<leadsto> \<epsilon> \<cdot> v\<^sub>1"
+| ev_snd [simp]: "\<Lambda> \<turnstile> \<pi>\<^sub>2 \<cdot> PairV v\<^sub>1 v\<^sub>2 \<leadsto> \<epsilon> \<cdot> v\<^sub>2"
+| ev_pair1 [simp]: "\<Lambda> \<turnstile> f\<^sub>1 \<cdot> v\<^sub>1 \<leadsto> f\<^sub>1' \<cdot> v\<^sub>1' \<Longrightarrow> \<Lambda> \<turnstile> f\<^sub>1 \<parallel> f\<^sub>2 \<cdot> PairV v\<^sub>1 v\<^sub>2 \<leadsto> f\<^sub>1' \<parallel> f\<^sub>2 \<cdot> PairV v\<^sub>1' v\<^sub>2"
+| ev_pair2 [simp]: "\<Lambda> \<turnstile> f\<^sub>2 \<cdot> v\<^sub>2 \<leadsto> f\<^sub>2' \<cdot> v\<^sub>2' \<Longrightarrow> \<Lambda> \<turnstile> \<epsilon> \<parallel> f\<^sub>2 \<cdot> PairV v\<^sub>1 v\<^sub>2 \<leadsto> \<epsilon> \<parallel> f\<^sub>2' \<cdot> PairV v\<^sub>1 v\<^sub>2'"
+| ev_pair3 [simp]: "\<Lambda> \<turnstile> \<epsilon> \<parallel> \<epsilon> \<cdot> PairV v\<^sub>1 v\<^sub>2 \<leadsto> \<epsilon> \<cdot> PairV v\<^sub>1 v\<^sub>2"
+| ev_tup [simp]: "\<Lambda> \<turnstile> \<Theta> \<cdot> v \<leadsto> \<epsilon> \<cdot> PairV v v"
+| ev_inl [simp]: "\<Lambda> \<turnstile> \<iota>\<^sub>l \<cdot> v \<leadsto> \<epsilon> \<cdot> InlV v"
+| ev_inr [simp]: "\<Lambda> \<turnstile> \<iota>\<^sub>r \<cdot> v \<leadsto> \<epsilon> \<cdot> InrV v"
+| ev_strl [simp]: "\<Lambda> \<turnstile> \<Xi> \<cdot> InlV v \<leadsto> \<epsilon> \<cdot> v"
+| ev_strr [simp]: "\<Lambda> \<turnstile> \<Xi> \<cdot> InrV v \<leadsto> \<epsilon> \<cdot> v"
+| ev_csl [simp]: "\<Lambda> \<turnstile> f\<^sub>l \<bar> f\<^sub>r \<cdot> InlV v \<leadsto> (\<iota>\<^sub>l \<cdot> f\<^sub>l) \<cdot> v"
+| ev_csr [simp]: "\<Lambda> \<turnstile> f\<^sub>l \<bar> f\<^sub>r \<cdot> InrV v \<leadsto> (\<iota>\<^sub>r \<cdot> f\<^sub>r) \<cdot> v"
+| ev_dstl [simp]: "\<Lambda> \<turnstile> \<rhd> \<cdot> PairV (InlV v\<^sub>1) v\<^sub>2 \<leadsto> \<epsilon> \<cdot> InlV (PairV v\<^sub>1 v\<^sub>2)"
+| ev_dstr [simp]: "\<Lambda> \<turnstile> \<rhd> \<cdot> PairV (InrV v\<^sub>1) v\<^sub>2 \<leadsto> \<epsilon> \<cdot> InrV (PairV v\<^sub>1 v\<^sub>2)"
+| ev_app [simp]: "\<Lambda> \<turnstile> $ \<cdot> PairV (FunV e) v \<leadsto> e \<cdot> v"
+| ev_arr [simp]: "\<Lambda> \<turnstile> g \<leftarrow> f \<cdot> FunV e \<leadsto> \<epsilon> \<cdot> FunV (g \<cdot> e \<cdot> f)"
+| ev_inj [simp]: "\<Lambda> \<turnstile> \<succ>\<^bsub>F\<^esub> \<cdot> v \<leadsto> \<epsilon> \<cdot> InjV F v"
+| ev_outj [simp]: "\<Lambda> \<turnstile> \<prec>\<^bsub>F\<^esub> \<cdot> InjV F v \<leadsto> \<epsilon> \<cdot> v"
+| ev_cata [simp]: "\<Lambda> \<turnstile> \<lparr> f \<rparr>\<^bsub>F\<^esub> \<cdot> v \<leadsto> (f \<cdot> \<lparr> f \<rparr>\<^bsub>F\<^esub> \<bullet> F \<cdot> \<prec>\<^bsub>F\<^esub>) \<cdot> v"
+| ev_ana [simp]: "\<Lambda> \<turnstile> \<lbrakk> f \<rbrakk>\<^bsub>F\<^esub> \<cdot> v \<leadsto> (\<succ>\<^bsub>F\<^esub> \<cdot> \<lbrakk> f \<rbrakk>\<^bsub>F\<^esub> \<bullet> F \<cdot> f) \<cdot> v"
+| ev_var [simp]: "\<Lambda> \<turnstile> Var x \<cdot> v \<leadsto> \<Lambda> x \<cdot> v"
 
 (* safety *)
 
@@ -146,33 +153,33 @@ lemma canonical_arrow: "\<Gamma> \<turnstile> v : t\<^sub>1 \<hookrightarrow> t\
 lemma canonical_mu: "\<Gamma> \<turnstile> v : \<mu> F \<Longrightarrow> \<exists>v'. (\<Gamma> \<turnstile> v' : \<mu> F \<star> F) \<and> v = InjV F v'"
   by (cases \<Gamma> v "\<mu> F" rule: typecheck\<^sub>v.cases) simp_all
 
-theorem progress: "\<Gamma> \<turnstile> e : t\<^sub>1 \<rightarrow> t\<^sub>2 \<Longrightarrow> \<Gamma> \<turnstile> v : t\<^sub>1 \<Longrightarrow> e \<noteq> \<epsilon> \<Longrightarrow> \<exists>e' v'. e \<cdot> v \<leadsto> e' \<cdot> v'"
+theorem progress: "\<Gamma> \<turnstile> e : t\<^sub>1 \<rightarrow> t\<^sub>2 \<Longrightarrow> \<Gamma> \<turnstile> v : t\<^sub>1 \<Longrightarrow> e \<noteq> \<epsilon> \<Longrightarrow> \<exists>e' v'. \<Lambda> \<turnstile> e \<cdot> v \<leadsto> e' \<cdot> v'"
     and "\<Gamma> \<turnstile> v : t\<^sub>1 \<Longrightarrow> True"
   proof (induction \<Gamma> e t\<^sub>1 t\<^sub>2 arbitrary: v rule: typecheck\<^sub>e_typecheck\<^sub>v.inducts)
   case (tc_con \<Gamma> v\<^sub>2 t\<^sub>2 t\<^sub>1)
-    have "\<kappa> v\<^sub>2 \<cdot> v \<leadsto> \<epsilon> \<cdot> v\<^sub>2" by simp
+    have "\<Lambda> \<turnstile> \<kappa> v\<^sub>2 \<cdot> v \<leadsto> \<epsilon> \<cdot> v\<^sub>2" by simp
     thus ?case by fastforce
   next case (tc_comp \<Gamma> f t\<^sub>2 t\<^sub>3 g)
     thus ?case
       proof (cases "g = \<epsilon>")
       case True
-        hence "(f \<cdot> g) \<cdot> v \<leadsto> f \<cdot> v" by simp
+        hence "\<Lambda> \<turnstile> (f \<cdot> g) \<cdot> v \<leadsto> f \<cdot> v" by simp
         thus ?thesis by fastforce
       next case False
-        with tc_comp obtain g' v' where "g \<cdot> v \<leadsto> g' \<cdot> v'" by blast
-        with tc_comp have "(f \<cdot> g) \<cdot> v \<leadsto> (f \<cdot> g') \<cdot> v'" by simp
+        with tc_comp obtain g' v' where "\<Lambda> \<turnstile> g \<cdot> v \<leadsto> g' \<cdot> v'" by blast
+        with tc_comp have "\<Lambda> \<turnstile> (f \<cdot> g) \<cdot> v \<leadsto> (f \<cdot> g') \<cdot> v'" by simp
         thus ?thesis by fastforce
       qed
   next case tc_fst
     then obtain v\<^sub>1 v\<^sub>2 where "v = PairV v\<^sub>1 v\<^sub>2" using canonical_prod by blast
-    hence "\<pi>\<^sub>1 \<cdot> v \<leadsto> \<epsilon> \<cdot> v\<^sub>1" by simp
+    hence "\<Lambda> \<turnstile> \<pi>\<^sub>1 \<cdot> v \<leadsto> \<epsilon> \<cdot> v\<^sub>1" by simp
     thus ?case by fastforce
   next case tc_snd
     then obtain v\<^sub>1 v\<^sub>2 where "v = PairV v\<^sub>1 v\<^sub>2" using canonical_prod by blast
-    hence "\<pi>\<^sub>2 \<cdot> v \<leadsto> \<epsilon> \<cdot> v\<^sub>2" by simp
+    hence "\<Lambda> \<turnstile> \<pi>\<^sub>2 \<cdot> v \<leadsto> \<epsilon> \<cdot> v\<^sub>2" by simp
     thus ?case by fastforce
   next case tc_tup
-    hence "\<Theta> \<cdot> v \<leadsto> \<epsilon> \<cdot> PairV v v" by simp
+    hence "\<Lambda> \<turnstile> \<Theta> \<cdot> v \<leadsto> \<epsilon> \<cdot> PairV v v" by simp
     thus ?case by fastforce
   next case (tc_pair \<Gamma> f\<^sub>1 t\<^sub>1 t\<^sub>2 f\<^sub>2)
     then obtain v\<^sub>1 v\<^sub>2 where V: "v = PairV v\<^sub>1 v\<^sub>2" using canonical_prod by blast
@@ -182,33 +189,33 @@ theorem progress: "\<Gamma> \<turnstile> e : t\<^sub>1 \<rightarrow> t\<^sub>2 \
         thus ?thesis
           proof (cases "f\<^sub>2 = \<epsilon>")
           case True
-            have "\<epsilon> \<parallel> \<epsilon> \<cdot> PairV v\<^sub>1 v\<^sub>2 \<leadsto> \<epsilon> \<cdot> PairV v\<^sub>1 v\<^sub>2" by simp
+            have "\<Lambda> \<turnstile> \<epsilon> \<parallel> \<epsilon> \<cdot> PairV v\<^sub>1 v\<^sub>2 \<leadsto> \<epsilon> \<cdot> PairV v\<^sub>1 v\<^sub>2" by simp
             with T True V show ?thesis by fastforce
           next case False
-            with tc_pair V obtain f\<^sub>2' v\<^sub>2' where "f\<^sub>2 \<cdot> v\<^sub>2 \<leadsto> f\<^sub>2' \<cdot> v\<^sub>2'" by blast
-            hence "\<epsilon> \<parallel> f\<^sub>2 \<cdot> PairV v\<^sub>1 v\<^sub>2 \<leadsto> \<epsilon> \<parallel> f\<^sub>2' \<cdot> PairV v\<^sub>1 v\<^sub>2'" by simp
+            with tc_pair V obtain f\<^sub>2' v\<^sub>2' where "\<Lambda> \<turnstile> f\<^sub>2 \<cdot> v\<^sub>2 \<leadsto> f\<^sub>2' \<cdot> v\<^sub>2'" by blast
+            hence "\<Lambda> \<turnstile> \<epsilon> \<parallel> f\<^sub>2 \<cdot> PairV v\<^sub>1 v\<^sub>2 \<leadsto> \<epsilon> \<parallel> f\<^sub>2' \<cdot> PairV v\<^sub>1 v\<^sub>2'" by simp
             with True V show ?thesis by fastforce
           qed
       next case False
-        with tc_pair V obtain f\<^sub>1' v\<^sub>1' where "f\<^sub>1 \<cdot> v\<^sub>1 \<leadsto> f\<^sub>1' \<cdot> v\<^sub>1'" by blast    
-        hence "f\<^sub>1 \<parallel> f\<^sub>2 \<cdot> PairV v\<^sub>1 v\<^sub>2 \<leadsto> f\<^sub>1' \<parallel> f\<^sub>2 \<cdot> PairV v\<^sub>1' v\<^sub>2" by simp
+        with tc_pair V obtain f\<^sub>1' v\<^sub>1' where "\<Lambda> \<turnstile> f\<^sub>1 \<cdot> v\<^sub>1 \<leadsto> f\<^sub>1' \<cdot> v\<^sub>1'" by blast    
+        hence "\<Lambda> \<turnstile> f\<^sub>1 \<parallel> f\<^sub>2 \<cdot> PairV v\<^sub>1 v\<^sub>2 \<leadsto> f\<^sub>1' \<parallel> f\<^sub>2 \<cdot> PairV v\<^sub>1' v\<^sub>2" by simp
         with V show ?thesis by fastforce
       qed
   next case tc_inl
-    hence "\<iota>\<^sub>l \<cdot> v \<leadsto> \<epsilon> \<cdot> InlV v" by simp
+    hence "\<Lambda> \<turnstile> \<iota>\<^sub>l \<cdot> v \<leadsto> \<epsilon> \<cdot> InlV v" by simp
     thus ?case by fastforce
   next case tc_inr
-    hence "\<iota>\<^sub>r \<cdot> v \<leadsto> \<epsilon> \<cdot> InrV v" by simp
+    hence "\<Lambda> \<turnstile> \<iota>\<^sub>r \<cdot> v \<leadsto> \<epsilon> \<cdot> InrV v" by simp
     thus ?case by fastforce
   next case tc_str
     then obtain v' where V: "v = InlV v' \<or> v = InrV v'" using canonical_sum by blast
     thus ?case
       proof (cases "v = InlV v'")
       case True
-        hence "\<Xi> \<cdot> v \<leadsto> \<epsilon> \<cdot> v'" by simp
+        hence "\<Lambda> \<turnstile> \<Xi> \<cdot> v \<leadsto> \<epsilon> \<cdot> v'" by simp
         thus ?thesis by fastforce
       next case False
-        with V have "\<Xi> \<cdot> v \<leadsto> \<epsilon> \<cdot> v'" by simp
+        with V have "\<Lambda> \<turnstile> \<Xi> \<cdot> v \<leadsto> \<epsilon> \<cdot> v'" by simp
         thus ?thesis by fastforce
       qed
   next case (tc_case \<Gamma> f\<^sub>l t\<^sub>1 t\<^sub>3 f\<^sub>r)
@@ -216,10 +223,10 @@ theorem progress: "\<Gamma> \<turnstile> e : t\<^sub>1 \<rightarrow> t\<^sub>2 \
     thus ?case
       proof (cases "v = InlV v'")
       case True
-        hence "f\<^sub>l \<bar> f\<^sub>r \<cdot> v \<leadsto> (\<iota>\<^sub>l \<cdot> f\<^sub>l) \<cdot> v'" by simp
+        hence "\<Lambda> \<turnstile> f\<^sub>l \<bar> f\<^sub>r \<cdot> v \<leadsto> (\<iota>\<^sub>l \<cdot> f\<^sub>l) \<cdot> v'" by simp
         thus ?thesis by fastforce
       next case False
-        with V have "f\<^sub>l \<bar> f\<^sub>r \<cdot> v \<leadsto> (\<iota>\<^sub>r \<cdot> f\<^sub>r) \<cdot> v'" by simp
+        with V have "\<Lambda> \<turnstile> f\<^sub>l \<bar> f\<^sub>r \<cdot> v \<leadsto> (\<iota>\<^sub>r \<cdot> f\<^sub>r) \<cdot> v'" by simp
         thus ?thesis by fastforce
       qed
   next case tc_dst
@@ -228,179 +235,188 @@ theorem progress: "\<Gamma> \<turnstile> e : t\<^sub>1 \<rightarrow> t\<^sub>2 \
     thus ?case
       proof (cases "v = PairV (InlV v\<^sub>1) v\<^sub>2")
       case True
-        hence "\<rhd> \<cdot> v \<leadsto> \<epsilon> \<cdot> InlV (PairV v\<^sub>1 v\<^sub>2)" by simp
+        hence "\<Lambda> \<turnstile> \<rhd> \<cdot> v \<leadsto> \<epsilon> \<cdot> InlV (PairV v\<^sub>1 v\<^sub>2)" by simp
         thus ?thesis by fastforce
       next case False
-        with V have "\<rhd> \<cdot> v \<leadsto> \<epsilon> \<cdot> InrV (PairV v\<^sub>1 v\<^sub>2)" by simp
+        with V have "\<Lambda> \<turnstile> \<rhd> \<cdot> v \<leadsto> \<epsilon> \<cdot> InrV (PairV v\<^sub>1 v\<^sub>2)" by simp
         thus ?thesis by fastforce
       qed
   next case tc_app
     then obtain e v' where V: "v = PairV (FunV e) v'" using canonical_prod canonical_arrow by blast
-    moreover hence "$ \<cdot> v \<leadsto> e \<cdot> v'" by simp
+    moreover hence "\<Lambda> \<turnstile> $ \<cdot> v \<leadsto> e \<cdot> v'" by simp
     ultimately show ?case by fastforce
   next case (tc_arr \<Gamma> f t\<^sub>1 t\<^sub>2 g)
     then obtain e where "v = FunV e" using canonical_arrow by blast
-    moreover hence "g \<leftarrow> f \<cdot> FunV e \<leadsto> \<epsilon> \<cdot> FunV (g \<cdot> e \<cdot> f)" by simp
+    moreover hence "\<Lambda> \<turnstile> g \<leftarrow> f \<cdot> FunV e \<leadsto> \<epsilon> \<cdot> FunV (g \<cdot> e \<cdot> f)" by simp
     ultimately show ?case by fastforce
   next case (tc_inj \<Gamma> F)
-    hence "\<succ>\<^bsub>F\<^esub> \<cdot> v \<leadsto> \<epsilon> \<cdot> InjV F v" by simp
+    hence "\<Lambda> \<turnstile> \<succ>\<^bsub>F\<^esub> \<cdot> v \<leadsto> \<epsilon> \<cdot> InjV F v" by simp
     thus ?case by fastforce
   next case (tc_outj \<Gamma> F)
     then obtain v' where "v = InjV F v'" using canonical_mu by blast
-    moreover hence "\<prec>\<^bsub>F\<^esub> \<cdot> v \<leadsto> \<epsilon> \<cdot> v'" by simp
+    moreover hence "\<Lambda> \<turnstile> \<prec>\<^bsub>F\<^esub> \<cdot> v \<leadsto> \<epsilon> \<cdot> v'" by simp
     ultimately show ?case by fastforce
   next case (tc_cata \<Gamma> f t F)
-    hence "\<lparr> f \<rparr>\<^bsub>F\<^esub> \<cdot> v \<leadsto> (f \<cdot> \<lparr> f \<rparr>\<^bsub>F\<^esub> \<bullet> F \<cdot> \<prec>\<^bsub>F\<^esub>) \<cdot> v" by simp
+    hence "\<Lambda> \<turnstile> \<lparr> f \<rparr>\<^bsub>F\<^esub> \<cdot> v \<leadsto> (f \<cdot> \<lparr> f \<rparr>\<^bsub>F\<^esub> \<bullet> F \<cdot> \<prec>\<^bsub>F\<^esub>) \<cdot> v" by simp
     thus ?case by fastforce
   next case (tc_ana \<Gamma> f t F)
-    hence "\<lbrakk> f \<rbrakk>\<^bsub>F\<^esub> \<cdot> v \<leadsto> (\<succ>\<^bsub>F\<^esub> \<cdot> \<lbrakk> f \<rbrakk>\<^bsub>F\<^esub> \<bullet> F \<cdot> f) \<cdot> v" by simp
+    hence "\<Lambda> \<turnstile> \<lbrakk> f \<rbrakk>\<^bsub>F\<^esub> \<cdot> v \<leadsto> (\<succ>\<^bsub>F\<^esub> \<cdot> \<lbrakk> f \<rbrakk>\<^bsub>F\<^esub> \<bullet> F \<cdot> f) \<cdot> v" by simp
+    thus ?case by fastforce
+  next case (tc_var \<Gamma> x)
+    have "\<Lambda> \<turnstile> Var x \<cdot> v \<leadsto> \<Lambda> x \<cdot> v" by simp
     thus ?case by fastforce
   qed simp_all
 
 lemma [simp]: "\<Gamma> \<turnstile> e : t\<^sub>1 \<rightarrow> t\<^sub>2 \<Longrightarrow> \<Gamma> \<turnstile> e \<bullet> F : t\<^sub>1 \<star> F \<rightarrow> t\<^sub>2 \<star> F"
   by (induction e F rule: apply_functor_expr.induct) simp_all
 
-theorem preservation: "e \<cdot> v \<leadsto> e' \<cdot> v' \<Longrightarrow> \<Gamma> \<turnstile> e : t\<^sub>1 \<rightarrow> t\<^sub>2 \<Longrightarrow> \<Gamma> \<turnstile> v : t\<^sub>1 \<Longrightarrow> 
+theorem preservation: "\<Lambda> \<turnstile> e \<cdot> v \<leadsto> e' \<cdot> v' \<Longrightarrow> \<Gamma> \<turnstile> e : t\<^sub>1 \<rightarrow> t\<^sub>2 \<Longrightarrow> \<Gamma> \<turnstile> v : t\<^sub>1 \<Longrightarrow> \<Gamma> \<tturnstile> \<Lambda> \<Longrightarrow>
     \<exists>t\<^sub>3. (\<Gamma> \<turnstile> e' : t\<^sub>3 \<rightarrow> t\<^sub>2) \<and> (\<Gamma> \<turnstile> v' : t\<^sub>3)"
-  proof (induction e v e' v' arbitrary: t\<^sub>1 t\<^sub>2 rule: evaluate.induct)
-  case (ev_pair1 f\<^sub>1 v\<^sub>1 f\<^sub>1' v\<^sub>1' f\<^sub>2 v\<^sub>2)
+  proof (induction \<Lambda> e v e' v' arbitrary: t\<^sub>1 t\<^sub>2 rule: evaluate.induct)
+  case (ev_pair1 \<Lambda> f\<^sub>1 v\<^sub>1 f\<^sub>1' v\<^sub>1' f\<^sub>2 v\<^sub>2)
     then obtain t\<^sub>1\<^sub>1 t\<^sub>1\<^sub>2 t\<^sub>2\<^sub>1 t\<^sub>2\<^sub>2 t\<^sub>1\<^sub>1' where T: "(\<Gamma> \<turnstile> v\<^sub>1 : t\<^sub>1\<^sub>1) \<and> (\<Gamma> \<turnstile> v\<^sub>2 : t\<^sub>1\<^sub>2) \<and> 
       (\<Gamma> \<turnstile> f\<^sub>1 : t\<^sub>1\<^sub>1 \<rightarrow> t\<^sub>2\<^sub>1) \<and> (\<Gamma> \<turnstile> f\<^sub>2 : t\<^sub>1\<^sub>2 \<rightarrow> t\<^sub>2\<^sub>2) \<and> t\<^sub>1 = t\<^sub>1\<^sub>1 \<otimes> t\<^sub>1\<^sub>2 \<and> t\<^sub>2 = t\<^sub>2\<^sub>1 \<otimes> t\<^sub>2\<^sub>2 \<and> 
         (\<Gamma> \<turnstile> f\<^sub>1' : t\<^sub>1\<^sub>1' \<rightarrow> t\<^sub>2\<^sub>1) \<and> \<Gamma> \<turnstile> v\<^sub>1' : t\<^sub>1\<^sub>1'" by fastforce
     hence "(\<Gamma> \<turnstile> f\<^sub>1' \<parallel> f\<^sub>2 : t\<^sub>1\<^sub>1' \<otimes> t\<^sub>1\<^sub>2 \<rightarrow> t\<^sub>2) \<and> \<Gamma> \<turnstile> PairV v\<^sub>1' v\<^sub>2 : t\<^sub>1\<^sub>1' \<otimes> t\<^sub>1\<^sub>2" by simp
     thus ?case by fastforce
-  next case (ev_pair2 f\<^sub>2 v\<^sub>2 f\<^sub>2' v\<^sub>2' v\<^sub>1)
+  next case (ev_pair2 \<Lambda> f\<^sub>2 v\<^sub>2 f\<^sub>2' v\<^sub>2' v\<^sub>1)
     then obtain t\<^sub>1\<^sub>1 t\<^sub>1\<^sub>2 t\<^sub>2\<^sub>2 t\<^sub>1\<^sub>2' where T: "(\<Gamma> \<turnstile> v\<^sub>1 : t\<^sub>1\<^sub>1) \<and> (\<Gamma> \<turnstile> v\<^sub>2 : t\<^sub>1\<^sub>2) \<and> (\<Gamma> \<turnstile> f\<^sub>2 : t\<^sub>1\<^sub>2 \<rightarrow> t\<^sub>2\<^sub>2) \<and> 
       t\<^sub>1 = t\<^sub>1\<^sub>1 \<otimes> t\<^sub>1\<^sub>2 \<and> t\<^sub>2 = t\<^sub>1\<^sub>1 \<otimes> t\<^sub>2\<^sub>2 \<and> (\<Gamma> \<turnstile> f\<^sub>2' : t\<^sub>1\<^sub>2' \<rightarrow> t\<^sub>2\<^sub>2) \<and> \<Gamma> \<turnstile> v\<^sub>2' : t\<^sub>1\<^sub>2'" by fastforce
     hence "(\<Gamma> \<turnstile> \<epsilon> \<parallel> f\<^sub>2' : t\<^sub>1\<^sub>1 \<otimes> t\<^sub>1\<^sub>2' \<rightarrow> t\<^sub>2) \<and> \<Gamma> \<turnstile> PairV v\<^sub>1 v\<^sub>2' : t\<^sub>1\<^sub>1 \<otimes> t\<^sub>1\<^sub>2'" by simp
     thus ?case by fastforce
-  next case (ev_tup v)
+  next case (ev_tup \<Lambda> v)
     hence "t\<^sub>2 = t\<^sub>1 \<otimes> t\<^sub>1" by fastforce
     moreover from ev_tup have "(\<Gamma> \<turnstile> \<epsilon> : t\<^sub>1 \<otimes> t\<^sub>1 \<rightarrow> t\<^sub>1 \<otimes> t\<^sub>1) \<and> \<Gamma> \<turnstile> PairV v v : t\<^sub>1 \<otimes> t\<^sub>1" by simp
     ultimately show ?case by fastforce
-  next case (ev_inl v)
+  next case (ev_inl \<Lambda> v)
     moreover then obtain t\<^sub>3 where "t\<^sub>2 = t\<^sub>1 \<oplus> t\<^sub>3" by fastforce
     ultimately have "(\<Gamma> \<turnstile> \<epsilon> : t\<^sub>1 \<oplus> t\<^sub>3 \<rightarrow> t\<^sub>2) \<and> \<Gamma> \<turnstile> InlV v : t\<^sub>1 \<oplus> t\<^sub>3" by simp
     thus ?case by fastforce
-  next case (ev_inr v)
+  next case (ev_inr \<Lambda> v)
     moreover then obtain t\<^sub>3 where "t\<^sub>2 = t\<^sub>3 \<oplus> t\<^sub>1" by fastforce
     ultimately have "(\<Gamma> \<turnstile> \<epsilon> : t\<^sub>3 \<oplus> t\<^sub>1 \<rightarrow> t\<^sub>2) \<and> \<Gamma> \<turnstile> InrV v : t\<^sub>3 \<oplus> t\<^sub>1" by simp
     thus ?case by fastforce
-  next case (ev_csl f\<^sub>l f\<^sub>r v)
+  next case (ev_csl \<Lambda> f\<^sub>l f\<^sub>r v)
     then obtain t\<^sub>1\<^sub>l t\<^sub>1\<^sub>r t\<^sub>2\<^sub>l t\<^sub>2\<^sub>r where V: "(\<Gamma> \<turnstile> f\<^sub>l : t\<^sub>1\<^sub>l \<rightarrow> t\<^sub>2\<^sub>l) \<and> (\<Gamma> \<turnstile> f\<^sub>r : t\<^sub>1\<^sub>r \<rightarrow> t\<^sub>2\<^sub>r) \<and> 
       (\<Gamma> \<turnstile> v : t\<^sub>1\<^sub>l) \<and> t\<^sub>1 = t\<^sub>1\<^sub>l \<oplus> t\<^sub>1\<^sub>r \<and> t\<^sub>2 = t\<^sub>2\<^sub>l \<oplus> t\<^sub>2\<^sub>r" by fastforce
     hence "\<Gamma> \<turnstile> \<iota>\<^sub>l \<cdot> f\<^sub>l : t\<^sub>1\<^sub>l \<rightarrow> t\<^sub>2\<^sub>l \<oplus> t\<^sub>2\<^sub>r" by (metis tc_inl tc_comp)
     with V show ?case by fastforce
-  next case (ev_csr f\<^sub>l f\<^sub>r v)
+  next case (ev_csr \<Lambda> f\<^sub>l f\<^sub>r v)
     then obtain t\<^sub>1\<^sub>l t\<^sub>1\<^sub>r t\<^sub>2\<^sub>l t\<^sub>2\<^sub>r where V: "(\<Gamma> \<turnstile> f\<^sub>l : t\<^sub>1\<^sub>l \<rightarrow> t\<^sub>2\<^sub>l) \<and> (\<Gamma> \<turnstile> f\<^sub>r : t\<^sub>1\<^sub>r \<rightarrow> t\<^sub>2\<^sub>r) \<and> 
       (\<Gamma> \<turnstile> v : t\<^sub>1\<^sub>r) \<and> t\<^sub>1 = t\<^sub>1\<^sub>l \<oplus> t\<^sub>1\<^sub>r \<and> t\<^sub>2 = t\<^sub>2\<^sub>l \<oplus> t\<^sub>2\<^sub>r" by fastforce
     hence "\<Gamma> \<turnstile> \<iota>\<^sub>r \<cdot> f\<^sub>r : t\<^sub>1\<^sub>r \<rightarrow> t\<^sub>2\<^sub>l \<oplus> t\<^sub>2\<^sub>r" by (metis tc_inr tc_comp)
     with V show ?case by fastforce
-  next case (ev_dstl v\<^sub>1 v\<^sub>2)
+  next case (ev_dstl \<Lambda> v\<^sub>1 v\<^sub>2)
     then obtain t\<^sub>3 t\<^sub>4 t\<^sub>5 where "(\<Gamma> \<turnstile> v\<^sub>1 : t\<^sub>3) \<and> (\<Gamma> \<turnstile> v\<^sub>2 : t\<^sub>5) \<and> t\<^sub>1 = (t\<^sub>3 \<oplus> t\<^sub>4) \<otimes> t\<^sub>5 \<and> 
       t\<^sub>2 = t\<^sub>3 \<otimes> t\<^sub>5 \<oplus> t\<^sub>4 \<otimes> t\<^sub>5" by fastforce
     hence "(\<Gamma> \<turnstile> \<epsilon> : t\<^sub>2 \<rightarrow> t\<^sub>2) \<and> \<Gamma> \<turnstile> InlV (PairV v\<^sub>1 v\<^sub>2) : t\<^sub>2" by simp
     thus ?case by fastforce
-  next case (ev_dstr v\<^sub>1 v\<^sub>2)
+  next case (ev_dstr \<Lambda> v\<^sub>1 v\<^sub>2)
     then obtain t\<^sub>3 t\<^sub>4 t\<^sub>5 where "(\<Gamma> \<turnstile> v\<^sub>1 : t\<^sub>4) \<and> (\<Gamma> \<turnstile> v\<^sub>2 : t\<^sub>5) \<and> t\<^sub>1 = (t\<^sub>3 \<oplus> t\<^sub>4) \<otimes> t\<^sub>5 \<and> 
       t\<^sub>2 = t\<^sub>3 \<otimes> t\<^sub>5 \<oplus> t\<^sub>4 \<otimes> t\<^sub>5" by fastforce
     hence "(\<Gamma> \<turnstile> \<epsilon> : t\<^sub>2 \<rightarrow> t\<^sub>2) \<and> \<Gamma> \<turnstile> InrV (PairV v\<^sub>1 v\<^sub>2) : t\<^sub>2" by simp
     thus ?case by fastforce
-  next case (ev_arr g f e)
+  next case (ev_arr \<Lambda> g f e)
     then obtain t\<^sub>1\<^sub>1 t\<^sub>1\<^sub>2 t\<^sub>2\<^sub>1 t\<^sub>2\<^sub>2 where "(\<Gamma> \<turnstile> f : t\<^sub>2\<^sub>1 \<rightarrow> t\<^sub>1\<^sub>1) \<and> (\<Gamma> \<turnstile> g : t\<^sub>1\<^sub>2 \<rightarrow> t\<^sub>2\<^sub>2) \<and> 
       (\<Gamma> \<turnstile> e : t\<^sub>1\<^sub>1 \<rightarrow> t\<^sub>1\<^sub>2) \<and> t\<^sub>1 = t\<^sub>1\<^sub>1 \<hookrightarrow> t\<^sub>1\<^sub>2 \<and> t\<^sub>2 = t\<^sub>2\<^sub>1 \<hookrightarrow> t\<^sub>2\<^sub>2" by fastforce
     hence "(\<Gamma> \<turnstile> \<epsilon> : t\<^sub>2\<^sub>1 \<hookrightarrow> t\<^sub>2\<^sub>2 \<rightarrow> t\<^sub>2) \<and> \<Gamma> \<turnstile> FunV (g \<cdot> e \<cdot> f) : t\<^sub>2\<^sub>1 \<hookrightarrow> t\<^sub>2\<^sub>2" by fastforce
     thus ?case by fastforce
-  next case (ev_inj F v)
+  next case (ev_inj \<Lambda> F v)
     hence "(\<Gamma> \<turnstile> \<epsilon> : t\<^sub>2 \<rightarrow> t\<^sub>2) \<and> \<Gamma> \<turnstile> InjV F v : t\<^sub>2" by fastforce
     thus ?case by fastforce
-  next case (ev_cata f F v)
+  next case (ev_cata \<Lambda> f F v)
     hence V: "(\<Gamma> \<turnstile> f : t\<^sub>2 \<star> F \<rightarrow> t\<^sub>2) \<and> \<Gamma> \<turnstile> v : \<mu> F" by fastforce
     moreover from ev_cata have "\<Gamma> \<turnstile> \<lparr> f \<rparr>\<^bsub>F\<^esub> \<bullet> F : \<mu> F \<star> F \<rightarrow> t\<^sub>2 \<star> F" by fastforce
     moreover have "\<Gamma> \<turnstile> \<prec>\<^bsub>F\<^esub> : \<mu> F \<rightarrow> \<mu> F \<star> F" by simp
     ultimately have "\<Gamma> \<turnstile> f \<cdot> \<lparr> f \<rparr>\<^bsub>F\<^esub> \<bullet> F \<cdot> \<prec>\<^bsub>F\<^esub> : \<mu> F \<rightarrow> t\<^sub>2" by (metis tc_comp)
     with V have "(\<Gamma> \<turnstile> f \<cdot> \<lparr> f \<rparr>\<^bsub>F\<^esub> \<bullet> F \<cdot> \<prec>\<^bsub>F\<^esub> : \<mu> F \<rightarrow> t\<^sub>2) \<and> \<Gamma> \<turnstile> v : \<mu> F" by simp
     thus ?case by fastforce
-  next case (ev_ana f F v)
+  next case (ev_ana \<Lambda> f F v)
     hence V: "(\<Gamma> \<turnstile> f : t\<^sub>1 \<rightarrow> t\<^sub>1 \<star> F) \<and> (\<Gamma> \<turnstile> v : t\<^sub>1) \<and> t\<^sub>2 = \<mu> F" by fastforce
     hence "\<Gamma> \<turnstile> \<succ>\<^bsub>F\<^esub> : t\<^sub>2 \<star> F \<rightarrow> t\<^sub>2" by simp
     moreover from ev_ana have "\<Gamma> \<turnstile> \<lbrakk> f \<rbrakk>\<^bsub>F\<^esub> \<bullet> F : t\<^sub>1 \<star> F \<rightarrow> t\<^sub>2 \<star> F" by simp
     moreover from V have "\<Gamma> \<turnstile> f : t\<^sub>1 \<rightarrow> t\<^sub>1 \<star> F" by simp
     ultimately have "\<Gamma> \<turnstile> \<succ>\<^bsub>F\<^esub> \<cdot> \<lbrakk> f \<rbrakk>\<^bsub>F\<^esub> \<bullet> F \<cdot> f : t\<^sub>1 \<rightarrow> t\<^sub>2" by simp
     with V show ?case by fastforce
+  next case (ev_var \<Lambda> x v)
+    moreover hence "\<Gamma> x = (t\<^sub>1, t\<^sub>2)" by fastforce
+    ultimately have "\<Gamma> \<turnstile> \<Lambda> x : t\<^sub>1 \<rightarrow> t\<^sub>2" by (simp add: typecheck_context_def)
+    with ev_var show ?case by fastforce
   qed force+
 
 (* big-step evaluation *) 
 
-inductive total_eval :: "expr \<Rightarrow> val \<Rightarrow> val \<Rightarrow> bool" (infix "\<cdot> _ \<Down>" 60) where
-  tev_base [simp]: "\<epsilon> \<cdot> v \<Down> v"
-| tev_step [simp]: "e \<cdot> v \<leadsto> e' \<cdot> v' \<Longrightarrow> e' \<cdot> v' \<Down> v'' \<Longrightarrow> e \<cdot> v \<Down> v''"
+inductive total_eval :: "(name \<Rightarrow> expr) \<Rightarrow> expr \<Rightarrow> val \<Rightarrow> val \<Rightarrow> bool" (infix "\<turnstile> _ \<cdot> _ \<Down>" 60) where
+  tev_base [simp]: "\<Lambda> \<turnstile> \<epsilon> \<cdot> v \<Down> v"
+| tev_step [simp]: "\<Lambda> \<turnstile> e \<cdot> v \<leadsto> e' \<cdot> v' \<Longrightarrow> \<Lambda> \<turnstile> e' \<cdot> v' \<Down> v'' \<Longrightarrow> \<Lambda> \<turnstile> e \<cdot> v \<Down> v''"
 
-lemma [elim]: "f \<cdot> v \<Down> v' \<Longrightarrow> g \<cdot> v' \<Down> v'' \<Longrightarrow> (g \<cdot> f) \<cdot> v \<Down> v''"
-  proof (induction f v v' rule: total_eval.induct)
-  case (tev_base v)
-    moreover have "(g \<cdot> \<epsilon>) \<cdot> v \<leadsto> g \<cdot> v" by simp
+lemma [elim]: "\<Lambda> \<turnstile> f \<cdot> v \<Down> v' \<Longrightarrow> \<Lambda> \<turnstile> g \<cdot> v' \<Down> v'' \<Longrightarrow> \<Lambda> \<turnstile> (g \<cdot> f) \<cdot> v \<Down> v''"
+  proof (induction \<Lambda> f v v' rule: total_eval.induct)
+  case (tev_base \<Lambda> v)
+    moreover have "\<Lambda> \<turnstile> (g \<cdot> \<epsilon>) \<cdot> v \<leadsto> g \<cdot> v" by simp
     ultimately show ?case by (metis tev_step)
-  next case (tev_step f v f' v' v''')
-    hence "(g \<cdot> f) \<cdot> v \<leadsto> (g \<cdot> f') \<cdot> v'" by simp
-    moreover from tev_step have "(g \<cdot> f') \<cdot> v' \<Down> v''" by simp
+  next case (tev_step \<Lambda> f v f' v' v''')
+    hence "\<Lambda> \<turnstile> (g \<cdot> f) \<cdot> v \<leadsto> (g \<cdot> f') \<cdot> v'" by simp
+    moreover from tev_step have "\<Lambda> \<turnstile> (g \<cdot> f') \<cdot> v' \<Down> v''" by simp
     ultimately show ?case by (metis total_eval.tev_step)
   qed
 
-lemma [simp]: "e \<cdot> v \<leadsto> \<epsilon> \<cdot> v' \<Longrightarrow> e \<cdot> v \<Down> v'"
+lemma [simp]: "\<Lambda> \<turnstile> e \<cdot> v \<leadsto> \<epsilon> \<cdot> v' \<Longrightarrow> \<Lambda> \<turnstile> e \<cdot> v \<Down> v'"
   by rule (simp, simp)
 
-lemma eps_big_eval [elim]: "\<epsilon> \<cdot> v \<Down> v' \<Longrightarrow> v = v'"
-  proof (induction \<epsilon> v v' rule: total_eval.induct)
-  case (tev_step v e' v' v'')
+lemma eps_big_eval [elim]: "\<Lambda> \<turnstile> \<epsilon> \<cdot> v \<Down> v' \<Longrightarrow> v = v'"
+  proof (induction \<Lambda> \<epsilon> v v' rule: total_eval.induct)
+  case (tev_step \<Lambda> v e' v' v'')
     thus ?case by (induction \<epsilon> v e' v' rule: evaluate.induct)
   qed simp_all
 
-lemma [simp]: "f\<^sub>2 \<cdot> v\<^sub>2 \<Down> v\<^sub>4 \<Longrightarrow> \<epsilon> \<parallel> f\<^sub>2 \<cdot> PairV v\<^sub>1 v\<^sub>2 \<Down> PairV v\<^sub>1 v\<^sub>4"
-  proof (induction f\<^sub>2 v\<^sub>2 v\<^sub>4 rule: total_eval.induct)
-  case (tev_step f\<^sub>2 v\<^sub>2 f\<^sub>2' v\<^sub>2' v\<^sub>4)
-    hence "\<epsilon> \<parallel> f\<^sub>2 \<cdot> PairV v\<^sub>1 v\<^sub>2 \<leadsto> \<epsilon> \<parallel> f\<^sub>2' \<cdot> PairV v\<^sub>1 v\<^sub>2'" by simp
-    moreover from tev_step have "\<epsilon> \<parallel> f\<^sub>2' \<cdot> PairV v\<^sub>1 v\<^sub>2' \<Down> PairV v\<^sub>1 v\<^sub>4" by simp
+lemma [simp]: "\<Lambda> \<turnstile> f\<^sub>2 \<cdot> v\<^sub>2 \<Down> v\<^sub>4 \<Longrightarrow> \<Lambda> \<turnstile> \<epsilon> \<parallel> f\<^sub>2 \<cdot> PairV v\<^sub>1 v\<^sub>2 \<Down> PairV v\<^sub>1 v\<^sub>4"
+  proof (induction \<Lambda> f\<^sub>2 v\<^sub>2 v\<^sub>4 rule: total_eval.induct)
+  case (tev_step \<Lambda> f\<^sub>2 v\<^sub>2 f\<^sub>2' v\<^sub>2' v\<^sub>4)
+    hence "\<Lambda> \<turnstile> \<epsilon> \<parallel> f\<^sub>2 \<cdot> PairV v\<^sub>1 v\<^sub>2 \<leadsto> \<epsilon> \<parallel> f\<^sub>2' \<cdot> PairV v\<^sub>1 v\<^sub>2'" by simp
+    moreover from tev_step have "\<Lambda> \<turnstile> \<epsilon> \<parallel> f\<^sub>2' \<cdot> PairV v\<^sub>1 v\<^sub>2' \<Down> PairV v\<^sub>1 v\<^sub>4" by simp
     ultimately show ?case by simp
   qed simp_all
 
-lemma [simp]: "f\<^sub>1 \<cdot> v\<^sub>1 \<Down> v\<^sub>3 \<Longrightarrow> f\<^sub>2 \<cdot> v\<^sub>2 \<Down> v\<^sub>4 \<Longrightarrow> f\<^sub>1 \<parallel> f\<^sub>2 \<cdot> PairV v\<^sub>1 v\<^sub>2 \<Down> PairV v\<^sub>3 v\<^sub>4"
-  proof (induction f\<^sub>1 v\<^sub>1 v\<^sub>3 rule: total_eval.induct)
-  case (tev_step f\<^sub>1 v\<^sub>1 f\<^sub>1' v\<^sub>1' v\<^sub>3)
-    hence "f\<^sub>1 \<parallel> f\<^sub>2 \<cdot> PairV v\<^sub>1 v\<^sub>2 \<leadsto> f\<^sub>1' \<parallel> f\<^sub>2 \<cdot> PairV v\<^sub>1' v\<^sub>2" by simp
-    moreover from tev_step have "f\<^sub>1' \<parallel> f\<^sub>2 \<cdot> PairV v\<^sub>1' v\<^sub>2 \<Down> PairV v\<^sub>3 v\<^sub>4" by simp
+lemma [simp]: "\<Lambda> \<turnstile> f\<^sub>1 \<cdot> v\<^sub>1 \<Down> v\<^sub>3 \<Longrightarrow> \<Lambda> \<turnstile> f\<^sub>2 \<cdot> v\<^sub>2 \<Down> v\<^sub>4 \<Longrightarrow> \<Lambda> \<turnstile> f\<^sub>1 \<parallel> f\<^sub>2 \<cdot> PairV v\<^sub>1 v\<^sub>2 \<Down> PairV v\<^sub>3 v\<^sub>4"
+  proof (induction \<Lambda> f\<^sub>1 v\<^sub>1 v\<^sub>3 rule: total_eval.induct)
+  case (tev_step \<Lambda> f\<^sub>1 v\<^sub>1 f\<^sub>1' v\<^sub>1' v\<^sub>3)
+    hence "\<Lambda> \<turnstile> f\<^sub>1 \<parallel> f\<^sub>2 \<cdot> PairV v\<^sub>1 v\<^sub>2 \<leadsto> f\<^sub>1' \<parallel> f\<^sub>2 \<cdot> PairV v\<^sub>1' v\<^sub>2" by simp
+    moreover from tev_step have "\<Lambda> \<turnstile> f\<^sub>1' \<parallel> f\<^sub>2 \<cdot> PairV v\<^sub>1' v\<^sub>2 \<Down> PairV v\<^sub>3 v\<^sub>4" by simp
     ultimately show ?case by simp
   qed simp_all
 
-lemma pair_big_eval [elim]: "f\<^sub>1 \<parallel> f\<^sub>2 \<cdot> PairV v\<^sub>1 v\<^sub>2 \<Down> PairV v\<^sub>3 v\<^sub>4 \<Longrightarrow> (f\<^sub>1 \<cdot> v\<^sub>1 \<Down> v\<^sub>3) \<and> f\<^sub>2 \<cdot> v\<^sub>2 \<Down> v\<^sub>4"
-  proof (induction "f\<^sub>1 \<parallel> f\<^sub>2" "PairV v\<^sub>1 v\<^sub>2" "PairV v\<^sub>3 v\<^sub>4" 
+lemma pair_big_eval [elim]: "\<Lambda> \<turnstile> f\<^sub>1 \<parallel> f\<^sub>2 \<cdot> PairV v\<^sub>1 v\<^sub>2 \<Down> PairV v\<^sub>3 v\<^sub>4 \<Longrightarrow> 
+    (\<Lambda> \<turnstile> f\<^sub>1 \<cdot> v\<^sub>1 \<Down> v\<^sub>3) \<and> \<Lambda> \<turnstile> f\<^sub>2 \<cdot> v\<^sub>2 \<Down> v\<^sub>4"
+  proof (induction \<Lambda> "f\<^sub>1 \<parallel> f\<^sub>2" "PairV v\<^sub>1 v\<^sub>2" "PairV v\<^sub>3 v\<^sub>4" 
          arbitrary: f\<^sub>1 f\<^sub>2 v\<^sub>1 v\<^sub>2 rule: total_eval.induct)
-  case (tev_step e' v')
+  case (tev_step \<Lambda> e' v')
     thus ?case
-      proof (induction "f\<^sub>1 \<parallel> f\<^sub>2" "PairV v\<^sub>1 v\<^sub>2" e' v' arbitrary: f\<^sub>1 f\<^sub>2 v\<^sub>1 v\<^sub>2 rule: evaluate.induct)
-      case (ev_pair3 v\<^sub>1 v\<^sub>2)
+      proof (induction \<Lambda> "f\<^sub>1 \<parallel> f\<^sub>2" "PairV v\<^sub>1 v\<^sub>2" e' v' arbitrary: f\<^sub>1 f\<^sub>2 v\<^sub>1 v\<^sub>2 rule: evaluate.induct)
+      case (ev_pair3 \<Lambda> v\<^sub>1 v\<^sub>2)
         hence "PairV v\<^sub>1 v\<^sub>2 = PairV v\<^sub>3 v\<^sub>4" by (metis eps_big_eval)
         thus ?case by simp
       qed simp_all
   qed
 
-lemma [simp]: "f\<^sub>l \<cdot> v \<Down> v' \<Longrightarrow> f\<^sub>l \<bar> f\<^sub>r \<cdot> InlV v \<Down> InlV v'"
+lemma [simp]: "\<Lambda> \<turnstile> f\<^sub>l \<cdot> v \<Down> v' \<Longrightarrow> \<Lambda> \<turnstile> f\<^sub>l \<bar> f\<^sub>r \<cdot> InlV v \<Down> InlV v'"
   proof
-    show "f\<^sub>l \<bar> f\<^sub>r \<cdot> InlV v \<leadsto> (\<iota>\<^sub>l \<cdot> f\<^sub>l) \<cdot> v" by simp
-    show "f\<^sub>l \<cdot> v \<Down> v' \<Longrightarrow> (\<iota>\<^sub>l \<cdot> f\<^sub>l) \<cdot> v \<Down> InlV v'" by auto
+    show "\<Lambda> \<turnstile> f\<^sub>l \<bar> f\<^sub>r \<cdot> InlV v \<leadsto> (\<iota>\<^sub>l \<cdot> f\<^sub>l) \<cdot> v" by simp
+    show "\<Lambda> \<turnstile> f\<^sub>l \<cdot> v \<Down> v' \<Longrightarrow> \<Lambda> \<turnstile> (\<iota>\<^sub>l \<cdot> f\<^sub>l) \<cdot> v \<Down> InlV v'" by auto
   qed
 
-lemma [simp]: "f\<^sub>r \<cdot> v \<Down> v' \<Longrightarrow> f\<^sub>l \<bar> f\<^sub>r \<cdot> InrV v \<Down> InrV v'"
+lemma [simp]: "\<Lambda> \<turnstile> f\<^sub>r \<cdot> v \<Down> v' \<Longrightarrow> \<Lambda> \<turnstile> f\<^sub>l \<bar> f\<^sub>r \<cdot> InrV v \<Down> InrV v'"
   proof
-    show "f\<^sub>l \<bar> f\<^sub>r \<cdot> InrV v \<leadsto> (\<iota>\<^sub>r \<cdot> f\<^sub>r) \<cdot> v" by simp
-    show "f\<^sub>r \<cdot> v \<Down> v' \<Longrightarrow> (\<iota>\<^sub>r \<cdot> f\<^sub>r) \<cdot> v \<Down> InrV v'" by auto
+    show "\<Lambda> \<turnstile> f\<^sub>l \<bar> f\<^sub>r \<cdot> InrV v \<leadsto> (\<iota>\<^sub>r \<cdot> f\<^sub>r) \<cdot> v" by simp
+    show "\<Lambda> \<turnstile> f\<^sub>r \<cdot> v \<Down> v' \<Longrightarrow> \<Lambda> \<turnstile> (\<iota>\<^sub>r \<cdot> f\<^sub>r) \<cdot> v \<Down> InrV v'" by auto
   qed
 
 (* since we are a turing-complete language, total progress is not provable *)
 
-theorem total_preservation: "e \<cdot> v \<Down> v' \<Longrightarrow> \<Gamma> \<turnstile> e : t\<^sub>1 \<rightarrow> t\<^sub>2 \<Longrightarrow> \<Gamma> \<turnstile> v : t\<^sub>1 \<Longrightarrow> \<Gamma> \<turnstile> v' : t\<^sub>2"
-  proof (induction e v v' arbitrary: t\<^sub>1 rule: total_eval.induct)
-  case (tev_step e v e' v' v'')
+theorem total_preservation: "\<Lambda> \<turnstile> e \<cdot> v \<Down> v' \<Longrightarrow> \<Gamma> \<turnstile> e : t\<^sub>1 \<rightarrow> t\<^sub>2 \<Longrightarrow> \<Gamma> \<turnstile> v : t\<^sub>1 \<Longrightarrow> \<Gamma> \<tturnstile> \<Lambda> \<Longrightarrow> 
+    \<Gamma> \<turnstile> v' : t\<^sub>2"
+  proof (induction \<Lambda> e v v' arbitrary: t\<^sub>1 rule: total_eval.induct)
+  case (tev_step \<Lambda> e v e' v' v'')
     moreover then obtain t\<^sub>3 where "(\<Gamma> \<turnstile> e' : t\<^sub>3 \<rightarrow> t\<^sub>2) \<and> (\<Gamma> \<turnstile> v' : t\<^sub>3)" by (metis preservation)
     ultimately show ?case by fastforce
   qed auto
